



$$\underline{t} = \underline{n} \cdot \underline{\underline{\sigma}}$$

$$\underline{t}_1^+ = \underline{e}_1 \cdot \underline{\underline{\sigma}} = [\sigma_{11}, \sigma_{12}]^T$$

$$\underline{t}_1^- = -\underline{e}_1 \cdot \underline{\underline{\sigma}} = -[\sigma_{11}, \sigma_{12}]^T$$

$$\underline{t}_2^+ = \underline{e}_2 \cdot \underline{\underline{\sigma}} = [\sigma_{21}, \sigma_{22}]^T$$

$$\underline{t}_2^- = -\underline{e}_2 \cdot \underline{\underline{\sigma}} = -[\sigma_{21}, \sigma_{22}]^T$$